src/Program.v
@@ -1,56 +1,54 @@
-Require Import Coq.ZArith.BinInt.
 Require Import bbv.Word.
-Require Import riscv.RiscvBitWidths.
 Require Import riscv.util.NameWithEq.
-Require Import riscv.Decode.
+
+Class Alu(t: Set) := mkAlu {
+  (* arithmetic operations: *)
+  add: t -> t -> t;
+  sub: t -> t -> t;
+  mul: t -> t -> t;
+  div: t -> t -> t;
+  rem: t -> t -> t;
+
+  (* comparison operators: *)
+  signed_less_than: t -> t -> bool;
+  unsigned_less_than: t -> t -> bool;
+
+  (* logical operations: *)
+  shift_left: t -> t -> t;
+  shift_right_logic: t -> t -> t;
+  shift_right_arith: t -> t -> t;
+  bitwise_xor: t -> t -> t;
+  bitwise_or: t -> t -> t;
+  bitwise_and: t -> t -> t;
+}.
+
+Class IntegralConversion(t1 t2: Set) := mkIntegralConversion {
+  fromIntegral: t1 -> t2
+}.
 
 Section Riscv.
 
-  Context {B: RiscvBitWidths}.
-
   Context {Name: NameWithEq}. (* register name *)
-  Notation Reg := (@name Name).
-  Existing Instance eq_name_dec.
+  Notation Register := (@name Name).
 
-  Class RiscvState(M: Type -> Type) := mkRiscvState {
-    getRegister: Register -> M (word wXLEN);
-    setRegister: Register -> (word wXLEN) -> M unit;
+  Class RiscvState(M: Type -> Type){t: Set}{A: Alu t} := mkRiscvState {
+    getRegister: Register -> M t;
+    setRegister{s: Set}{c: IntegralConversion s t}: Register -> s -> M unit;
 
-    loadByte: Z -> M (word 8);
-    loadHalf: Z -> M (word 16);
-    loadWord: Z -> M (word 32);
-    loadDouble: Z -> M (word 64);
+    loadByte: t -> M (word 8);
+    loadHalf: t -> M (word 16);
+    loadWord: t -> M (word 32);
+    loadDouble: t -> M (word 64);
 
-    storeByte: Z -> (word 8) -> M unit;
-    storeHalf: Z -> (word 16) -> M unit;
-    storeWord: Z -> (word 32) -> M unit;
-    storeDouble: Z -> (word 64) -> M unit;
+    storeByte: t -> (word 8) -> M unit;
+    storeHalf: t -> (word 16) -> M unit;
+    storeWord: t -> (word 32) -> M unit;
+    storeDouble: t -> (word 64) -> M unit;
 
-    getPC: M (word wXLEN);
-    setPC: (word wXLEN) -> M unit;
+    getPC: M t;
+    setPC: t -> M unit;
 
     step: M unit; (* updates PC *)
   }.
-
-(* With word-based addresses:
-
-  Class RiscvState(M: Type -> Type) := mkRiscvState {
-    getRegister: Register -> M (word wXLEN);
-    setRegister: Register -> (word wXLEN) -> M unit;
-
-    loadByte: (word wXLEN) -> M (word 8);
-    loadHalf: (word wXLEN) -> M (word 16);
-    loadWord: (word wXLEN) -> M (word 32);
-    loadDouble: (word wXLEN) -> M (word 64);
-
-    storeByte: (word wXLEN) -> (word 8) -> M unit;
-    storeHalf: (word wXLEN) -> (word 16) -> M unit;
-    storeWord: (word wXLEN) -> (word 32) -> M unit;
-    storeDouble: (word wXLEN) -> (word 64) -> M unit;
-
-    getPC: M Z;
-    setPC: Z -> M unit;
-  }.
-*)
 
 End Riscv.
